updating grammar

IndexedExample.v
@@ -1,6 +1,16 @@
 Set Implicit Arguments.
 Require Import Coq.Lists.List.
  
+(* The class is if the information is sensitive. Red means sensitive *)
+Inductive class : Type :=
+| red : class
+| green : class.
+
+(* decidablility *)
+Definition eq_class_dec: forall x y:class, {x=y}+{x<>y}.
+Proof.
+repeat decide equality.
+Defined.
  (* 3 measurements 
    1. VC
    2. sign VC 
@@ -10,6 +20,7 @@ Require Import Coq.Lists.List.
  Inductive place : Type :=
  | AP : place
  | TP : place
+ | MP : place 
  | VC : place
  | SS : place
  | priv_key : place.
@@ -20,16 +31,6 @@ Require Import Coq.Lists.List.
  repeat decide equality.
  Defined.
  
-  (* The class is if the information is sensitive. Red means sensitive *)
- Inductive class : Type :=
- | red : class
- | green : class.
-
-  (* decidablility *)
-  Definition eq_class_dec: forall x y:class, {x=y}+{x<>y}.
-  Proof.
-  repeat decide equality.
-  Defined.
 
  (* here, the structure of evidence is a Set 
      https://ku-sldg.github.io/copland/resources/coplandcoq/html/Copland.Term.html *)
@@ -47,17 +48,20 @@ Require Import Coq.Lists.List.
  Fixpoint privPolicy tp (e:evidence tp): Prop :=
    match e with
    | EHash _ => True
-   | EBlob p c => match p with 
-                  | SS => False 
-                  | _ => True 
+   | EBlob p c => match p, c with 
+                  | SS, red => False 
+                  | SS, green => False 
+                  | _ , red => False
+                  | _ , green => True 
                   end
    | ESig _ e' _ => privPolicy e' 
-   | ECrypt rp e' tp => if (in_dec (eq_place_dec) tp good_encrypt) then (match e' with 
-                                                                  | EBlob priv_key red => False 
-                                                                  | EBlob _ red => True 
-                                                                  | _ => privPolicy e'
-                                                                  end) 
-                                                                    else privPolicy e'
+   | ECrypt rp e' tp => if (in_dec (eq_place_dec) tp good_encrypt) 
+                        then (match e' with 
+                                | EBlob priv_key red => False 
+                                | EBlob _ red => True 
+                                | _ => privPolicy e'
+                              end) 
+                        else privPolicy e'
    | ESeq _ l r => (privPolicy l) /\ (privPolicy r)
    | EPar _ l r => (privPolicy l) /\ (privPolicy r)
    end.
@@ -77,28 +81,44 @@ Require Import Coq.Lists.List.
      is asking for the measurment, ap.  
      
      -> privPolicy ap (EBlob p c)*)
-  Inductive term p : evidence p  -> Type :=
-  | TMeas : forall e,  privPolicy e -> term e
-  | THash : forall e, e -> term (EHash p)
-  | TSig :
-       forall e q, term e -> privPolicy (ESig p e q) -> term (ESig p e q)
-  | TCrypt :
-      forall (q : place) e , place -> term e -> privPolicy (ECrypt p e q) -> term (ECrypt p e q)
-  | TSeq : forall e f,
-      term e -> privPolicy e -> term f -> privPolicy f -> term (ESeq p e f)
-  | TPar : forall e f,
-      term e -> privPolicy e -> term f -> privPolicy f -> term (EPar p e f).
+    Inductive term p : evidence p  -> Type :=
+    | TMeas : forall c,  privPolicy (EBlob p c) -> term (EBlob p c)
+    | THash : term (EHash p)
+    | TSig :
+         forall e q, term e -> privPolicy (ESig p e q) -> term (ESig p e q)
+    | TCrypt :
+        forall e q, term e -> privPolicy (ECrypt p e q) -> term (ECrypt p e q)
+    | TSeq : forall e f,
+        term e -> privPolicy e -> term f -> privPolicy f -> term (ESeq p e f)
+    | TPar : forall e f,
+        term e -> privPolicy e -> term f -> privPolicy f -> term (EPar p e f).
 
    Lemma vc_green : privPolicy (EBlob VC green).
    Proof. unfold privPolicy. auto. Qed.
 
-   Definition vc := TMeas (EBlob VC green).
+   Definition vc := TMeas VC green.
    Check vc. (* : privPolicy (EBlob VC green) -> term (EBlob VC green) *)
-   Definition vc' := TMeas (EBlob VC green) vc_green.
+   Definition vc' := TMeas VC green vc_green.
    Check vc'. (*: term (EBlob VC green) *)
 
-   Definition vc_sig := TSig TP (TMeas (EBlob VC green) vc_green).
+   Definition vc_sig := TSig TP (TMeas VC green vc_green).
    
    Definition vc_ss := False.  (*this will be impossible to write... no proof that EBlob SS satisfies priv policy *)
    
+  Compute TCrypt AP ((TMeas TP red) _).
+  (* = fun x : privPolicy (ECrypt TP (EBlob TP red) AP) =>
+       TCrypt AP (TMeas TP red ?p) x
+     : privPolicy (ECrypt TP (EBlob TP red) AP) ->
+       term (ECrypt TP (EBlob TP red) AP) *)
 
+  (*Definition crypt := TCrypt AP (TMeas TP red).*)
+  
+  
+  Lemma encrypt_okay : privPolicy (ECrypt TP (EBlob TP red) AP).
+  Proof. unfold privPolicy. simpl. auto. Qed.
+  Check encrypt_okay. 
+  
+  Compute TCrypt AP (TMeas TP red _) encrypt_okay.
+  
+  (* Definition ecrypt := TCrypt AP (TMeas TP red _) encrypt_okay.*)
+  
